q3

A1/Q3.dfy
@@ -12,20 +12,26 @@ function method pick (i: nat ): nat
     x + i * y
 }
 
-function method reverse (x: nat, y: nat): nat
-    decreases x
-{
-    if (x == 0 && y == 0) then 0 else
-        if (x > 0 && y >= 0) then 1 + reverse(x - 1, y + 1) else
-            if (x == 0 && y > 0) then 1 + reverse(y - 1, x) else 
-                0
-}
+// function method reverse (x: nat, y: nat): nat
+//     decreases x, y
+// {
+//     if (x == 0 && y == 0) then 0 else
+//         if (x > 0 && y >= 0) then 1 + reverse(x - 1, y + 1) else
+//             if (x == 0 && y > 0) then 1 + reverse(y - 1, x) else 
+//                 0
+// }
 
+function method reverse(a: nat , b: nat ): nat
+{
+    ((a + b) * (a + b + 1)) / 2 + a
+}
 
 lemma check(a: nat , b: nat, i: nat)
     requires a >= 0;
     requires b >= 0;
-    ensures exists x,y :: i == reverse(x, y) == reverse(a, b) ==> x == unpair(i).0 && y == unpair(i).1;
+    requires i >= 0;
+    ensures reverse(a, b) >= i;
+    ensures exists x, y :: i == reverse(x, y) == reverse(a, b) ==> x == unpair(i).0 && y == unpair(i).1;
 {
 
 }
